feat: Stlc fv

CollapsingTowers/Stlc/Basic.lean
@@ -1,7 +1,8 @@
 
+import Mathlib.Data.Finset.Basic
 inductive Expr : Type where
-  | bvar (i : Nat)
-  | fvar (x : String)
+  | bvar (i : ℕ)
+  | fvar (x : ℕ)
   | lam (e : Expr)
   | app (f : Expr) (arg : Expr)
   | unit
@@ -9,3 +10,11 @@ inductive Expr : Type where
 inductive value : Expr -> Prop where
   | value_lam : value (.lam e)
   | value_unit : value .unit
+
+@[simp]
+def fv : Expr → Finset ℕ
+  | .bvar _ => ∅
+  | .fvar y => { y }
+  | .lam e => fv e
+  | .app f arg => fv f ∪ fv arg
+  | .unit => ∅
